thys/Transport/HOL_Basics/Binary_Relations/Wellfounded_Recursion/Wellfounded_Recursion.thy
@@ -1,6 +1,6 @@
 \<^marker>\<open>creator "Kevin Kappelmann"\<close>
 \<^marker>\<open>creator "Niklas Krofta"\<close>
-section \<open>Well-Founded Recursion\<close>
+subsection \<open>Well-Founded Recursion\<close>
 theory Wellfounded_Recursion
   imports
     Binary_Relations_Transitive_Closure
@@ -8,9 +8,9 @@ theory Wellfounded_Recursion
 begin
 
 paragraph \<open>Summary\<close>
-text \<open>We use @{term wftrec} to define well-founded recursion on non-transitive, well-founded
+text \<open>We use @{term wft_rec} to define well-founded recursion on non-transitive, well-founded
 relations. The fact that the transitive closure of a well-founded relation is itself well-founded
-can be used to remove the transitivity assumption of @{thm wftrec_eq_wfrec_stepI}.\<close>
+can be used to remove the transitivity assumption of @{thm wft_rec_eq_wf_rec_stepI}.\<close>
 
 lemma wellfounded_trans_closure_if_wellfounded:
   assumes "wellfounded R"
@@ -18,7 +18,7 @@ lemma wellfounded_trans_closure_if_wellfounded:
 proof (rule ccontr)
   assume "\<not>(wellfounded (trans_closure R))"
   then obtain P X where "P X" and no_minimal: "\<And>Y. P Y \<Longrightarrow> (\<exists>y. trans_closure R y Y \<and> P y)"
-    unfolding wellfounded_rel_def by auto
+    unfolding wellfounded_eq_wellfounded_on wellfounded_on_pred_def by auto
   from assms have "\<not>(P Y) \<and> (\<forall>y. trans_closure R y Y \<longrightarrow> \<not>(P y))" for Y
   proof (induction Y rule: wellfounded_induct)
     case (step Y)
@@ -40,20 +40,54 @@ proof (rule ccontr)
   then show "False" using \<open>P X\<close> by blast
 qed
 
-definition "wfrec R step = wftrec (trans_closure R) (\<lambda>f. wfrec_step R step (\<lambda>_. f))"
+consts wf_rec :: "'a \<Rightarrow> 'b \<Rightarrow> 'c"
 
-theorem wfrec_eq_wfrec_stepI:
+definition "wf_rec_rel R step = wft_rec (trans_closure R) (\<lambda>f. wf_rec_step R step (\<lambda>_. f))"
+adhoc_overloading wf_rec wf_rec_rel
+
+theorem wf_rec_eq_wf_rec_stepI:
   assumes "wellfounded R"
-  shows "wfrec R step X = wfrec_step R step (\<lambda>_. wfrec R step) X"
+  shows "wf_rec R step X = wf_rec_step R step (\<lambda>_. wf_rec R step) X"
 proof -
   have fun_rel_restrict_eq:
     "fun_rel_restrict (fun_rel_restrict f (trans_closure R) X) R X x = fun_rel_restrict f R X x"
     for f x by (cases "R x X") (auto dest: trans_closure_if_rel)
-  have "wfrec R step X = wfrec_step R step (fun_rel_restrict (wfrec R step) (trans_closure R)) X"
+  have "wf_rec R step X = wf_rec_step R step (fun_rel_restrict (wf_rec R step) (trans_closure R)) X"
     using wellfounded_trans_closure_if_wellfounded[OF assms] transitive_trans_closure[of R]
-    wftrec_eq_wfrec_stepI[where ?step="\<lambda>f. wfrec_step R step (\<lambda>_. f)"]
-    by (simp add: wfrec_step_eq wfrec_def)
-  then show ?thesis unfolding wfrec_step_eq fun_rel_restrict_eq by simp
+    wft_rec_eq_wf_rec_stepI[where ?step="\<lambda>f. wf_rec_step R step (\<lambda>_. f)"]
+    by (simp add: wf_rec_step_eq wf_rec_rel_def)
+  then show ?thesis unfolding wf_rec_step_eq fun_rel_restrict_eq by simp
+qed
+
+consts wf_rec_on :: "'a \<Rightarrow> 'b \<Rightarrow> 'c \<Rightarrow> 'd"
+
+definition wf_rec_on_pred :: "('a \<Rightarrow> bool) \<Rightarrow> ('a \<Rightarrow> 'a \<Rightarrow> bool) \<Rightarrow> (('a \<Rightarrow> 'b) \<Rightarrow> 'a \<Rightarrow> 'b) \<Rightarrow> 'a \<Rightarrow> 'b" where
+  "wf_rec_on_pred P R \<equiv> wf_rec R\<up>\<^bsub>P\<^esub>"
+adhoc_overloading wf_rec_on wf_rec_on_pred
+
+lemma wf_rec_on_eq_wf_rec_restrict: "wf_rec_on P R = wf_rec R\<up>\<^bsub>P\<^esub>"
+  unfolding wf_rec_on_pred_def by simp
+
+theorem wf_rec_on_eq_wf_rec_step_restrictI:
+  assumes "wellfounded_on P R"
+  shows "wf_rec_on P R step X = wf_rec_step R\<up>\<^bsub>P\<^esub> step (\<lambda>_. wf_rec_on P R step) X"
+proof -
+  from assms have "wellfounded R\<up>\<^bsub>P\<^esub>" using wellfounded_rel_restrict_if_wellfounded_on by blast
+  with wf_rec_eq_wf_rec_stepI show ?thesis unfolding wf_rec_on_eq_wf_rec_restrict by fastforce
+qed
+
+lemma wf_rec_on_eq_app_fun_restrict_fun_rel_restrictI:
+  fixes step
+  assumes wf: "wellfounded_on P R"
+  and "P x"
+  defines "f \<equiv> wf_rec_on P R step"
+  shows "f x = step (fun_restrict (fun_rel_restrict f R x) P) x"
+proof -
+  from wf have "f x = step (fun_rel_restrict f R\<up>\<^bsub>P\<^esub> x) x"
+    unfolding f_def by (simp only: wf_rec_step_eq wf_rec_on_eq_wf_rec_step_restrictI)
+  moreover have "fun_rel_restrict f R\<up>\<^bsub>P\<^esub> x = fun_restrict (fun_rel_restrict f R x) P"
+    using \<open>P x\<close> fun_rel_restrict_rel_restrict_eq_fun_restrict_fun_rel_restrictI by simp
+  ultimately show ?thesis by simp
 qed
 
 
