thys/ML_Unification/Unifiers/ML_Unifiers.thy
@@ -53,15 +53,22 @@ declare [[ucombine add = \<open>Standard_Unification_Combine.eunif_data
   |> K)
   (Standard_Unification_Combine.metadata \<^binding>\<open>var_hop_unif\<close> Prio.HIGH)\<close>]]
 
-declare [[ucombine add = \<open>Standard_Unification_Combine.eunif_data
-  (Simplifier_Unification.simp_unify_progress Envir.aeconv Simplifier_Unification.simp_unify
-    (Unification_Util.inst_norm_term'
-      Standard_Mixed_Unification.norms_first_higherp_decomp_comb_higher_unify)
-    Standard_Mixed_Unification.norms_first_higherp_decomp_comb_higher_unify
-    Standard_Mixed_Unification.first_higherp_decomp_comb_higher_unify
-  |> Type_Unification.e_unify Unification_Util.unify_types
-  |> K)
-  (Standard_Unification_Combine.default_metadata \<^binding>\<open>simp_unif\<close>)
-  \<close>]]
+declare [[ucombine add = \<open>
+  let
+    open Term_Normalisation
+    (*ignore changes of schematic variables to avoid loops due to index-raising of some tactics*)
+    val eq_beta_eta_dummy_vars = apply2 (beta_eta_short #> dummy_vars) #> op aconv
+  in
+    Standard_Unification_Combine.eunif_data
+      (Simplifier_Unification.simp_unify_progress eq_beta_eta_dummy_vars
+        Simplifier_Unification.simp_unify
+        (Unification_Util.inst_norm_term'
+          Standard_Mixed_Unification.norms_first_higherp_decomp_comb_higher_unify)
+        Standard_Mixed_Unification.norms_first_higherp_decomp_comb_higher_unify
+        Standard_Mixed_Unification.first_higherp_decomp_comb_higher_unify
+      |> Type_Unification.e_unify Unification_Util.unify_types
+      |> K)
+      (Standard_Unification_Combine.default_metadata \<^binding>\<open>simp_unif\<close>)
+  end\<close>]]
 
 end
