thys/Transport/HOL_Basics/Binary_Relations/Properties/Binary_Relations_Antisymmetric.thy
@@ -3,6 +3,7 @@ subsubsection \<open>Antisymmetric\<close>
 theory Binary_Relations_Antisymmetric
   imports
     Binary_Relation_Functions
+    Functions_Monotone
 begin
 
 consts antisymmetric_on :: "'a \<Rightarrow> 'b \<Rightarrow> bool"
@@ -24,6 +25,15 @@ lemma antisymmetric_onD:
   and "R x y" "R y x"
   shows "x = y"
   using assms unfolding antisymmetric_on_pred_def by blast
+
+lemma antisymmetric_onE:
+  assumes "antisymmetric_on P R"
+  obtains "\<And>x y. P x \<Longrightarrow> P y \<Longrightarrow> R x y \<Longrightarrow> R y x \<Longrightarrow> x = y"
+  using assms unfolding antisymmetric_on_pred_def by blast
+
+lemma antimono_antisymmetric_on:
+  "((\<le>) \<Rightarrow> (\<le>) \<Rrightarrow> (\<ge>)) (antisymmetric_on :: ('a \<Rightarrow> bool) \<Rightarrow> ('a \<Rightarrow> 'a \<Rightarrow> bool) \<Rightarrow> bool)"
+  by (blast intro!: antisymmetric_onI dest: antisymmetric_onD)
 
 consts antisymmetric :: "'a \<Rightarrow> bool"
 
@@ -51,6 +61,11 @@ lemma antisymmetricD:
   and "R x y" "R y x"
   shows "x = y"
   using assms by (urule (d) antisymmetric_onD where chained = insert) simp_all
+
+lemma antisymmetricE:
+  assumes "antisymmetric R"
+  obtains "\<And>x y. R x y \<Longrightarrow> R y x \<Longrightarrow> x = y"
+  using assms by (urule (e) antisymmetric_onE where chained = insert) simp_all
 
 lemma antisymmetric_on_if_antisymmetric:
   fixes P :: "'a \<Rightarrow> bool" and R :: "'a \<Rightarrow> 'a \<Rightarrow> bool"
