thys/Transport/HOL_Basics/Binary_Relations/Properties/Binary_Relations_Connected.thy
@@ -3,6 +3,7 @@ subsubsection \<open>Connected\<close>
 theory Binary_Relations_Connected
   imports
     Binary_Relation_Functions
+    Functions_Injective
 begin
 
 consts connected_on :: "'a \<Rightarrow> 'b \<Rightarrow> bool"
@@ -27,6 +28,32 @@ lemma connected_onE [elim]:
 lemma connected_on_rel_inv_iff_connected_on [iff]:
   "connected_on (P :: 'a \<Rightarrow> bool) (R :: 'a \<Rightarrow> 'a \<Rightarrow> bool)\<inverse> \<longleftrightarrow> connected_on P R"
   by blast
+
+lemma connected_on_rel_map_if_injective_on_if_mono_wrt_pred_if_connected_on:
+  fixes P :: "'a \<Rightarrow> bool" and R :: "'a \<Rightarrow> 'a \<Rightarrow> bool"
+  assumes "connected_on P R"
+  and "(Q \<Rightarrow> P) f"
+  and "injective_on Q f"
+  shows "connected_on Q (rel_map f R)"
+  using assms by (fastforce dest: injective_onD)
+
+lemma antimono_connected_on: "antimono (connected_on :: ('a \<Rightarrow> bool) \<Rightarrow> ('a \<Rightarrow> 'a \<Rightarrow> bool) \<Rightarrow> bool)"
+  by (intro antimonoI) auto
+
+lemma mono_connected_on:
+  "((\<le>) \<Rightarrow> (\<ge>) \<Rrightarrow> (\<ge>)) (connected_on :: ('a \<Rightarrow> bool) \<Rightarrow> ('a \<Rightarrow> 'a \<Rightarrow> bool) \<Rightarrow> bool)"
+  by blast
+
+lemma in_field_restrict_eq_if_ex_ne_if_connected_on:
+  assumes conn: "connected_on P R"
+  and eq_ne: "\<exists>x y : P. x \<noteq> y"
+  shows "in_field R\<up>\<^bsub>P\<^esub> = P"
+proof (intro ext iffI)
+  fix x assume "P x"
+  moreover with eq_ne obtain y where "P y" "x \<noteq> y" by blast
+  ultimately have "R x y \<or> R y x" using conn by blast
+  with \<open>P x\<close> \<open>P y\<close> show "in_field R\<up>\<^bsub>P\<^esub> x" by fastforce
+qed auto
 
 consts connected :: "'a \<Rightarrow> bool"
 
